tests/lean/run/grind_offset_cnstr.lean
@@ -394,3 +394,11 @@ example (a : Nat) : a < 2 → a = 5 → False := by
 
 example (a : Nat) : a < 2 → a = b → b = c → c = 5 → False := by
   grind
+
+#guard_msgs (info) in -- none of the numerals should be internalized by the offset module
+set_option trace.grind.offset.internalize true in
+example (a b c d e : Nat) : a = 1 → b = 2 → c = 3 → d = 4 → e = 5 → a ≠ e := by
+  grind
+
+example (a b : Nat) : a + 1 = b → b = 0 → False := by
+  grind
